ocamllibs/dafny_examples/Example_sum.dfy
@@ -1,10 +1,13 @@
+function DfLength(s: seq<int>): int
+{if s == [] then 0 else DfLength(s[..|s|-1]) + 1}
+
 function Sum(a : seq<int>): int
 { if a == [] then  0 else  (Sum(a[..|a|-1]) + a[|a|-1]) 
 }
 
 function SumJoin(leftSum : int, rightSum : int): int
 {
-  (rightSum + leftSum)
+  ((rightSum - 1) + (leftSum - -1))
 }
 
 
@@ -19,7 +22,8 @@ lemma HomSum(a : seq<int>, R_a : seq<int>)
     {
     assert(a + [] == a);
     BaseCaseSum(a);
-    } else {
+    
+     } else {
     calc{
     Sum(a + R_a);
     =={ assert(a + R_a[..|R_a|-1]) + [R_a[|R_a|-1]] == a + R_a; }
