ocamllibs/dafny_examples/Is_sorted.dfy
@@ -1,0 +1,113 @@
+function DfLength(s: seq<int>): int
+{if s == [] then 0 else DfLength(s[..|s|-1]) + 1}
+
+function DfMax(x: int, y: int): int { if x > y then x else y}
+
+function DfMin(x: int, y: int): int { if x > y then y else x}
+
+function DfMinSeq(s : seq<int>) : int 
+  requires |s| >= 1
+{
+  if |s| == 1 then s[0]
+  else
+  DfMin(DfMinSeq(s[..|s|-1]), s[|s|-1])}function Aux_0(a : seq<int>): int
+requires |a| >= 1
+{ if |a| == 1 then  a[0] else  a[0] 
+}
+
+function Iss(a : seq<int>): bool
+{ if a == [] then
+    true
+   else 
+   (Iss(a[..|a|-1]) && (Prev(a[..|a|-1]) < a[|a|-1]))
+   
+}
+
+function Prev(a : seq<int>): int
+{ if a == [] then  DfMinSeq else  a[|a|-1] 
+}
+
+function Aux_0Join(leftAux_0 : int, rightAux_0 : int): int
+{
+  leftAux_0
+}
+
+function IssJoin(leftAux_0 : int, leftPrev : int, leftIss : bool, rightAux_0 : int, rightPrev : int, rightIss : bool): bool
+{
+  (((rightAux_0 - leftPrev) >= 1) && (leftIss && rightIss))
+}
+
+function PrevJoin(leftPrev : int, rightPrev : int): int
+{
+  DfMax(rightPrev, -2)
+}
+
+
+lemma HomAux_0(a : seq<int>, R_a : seq<int>)
+  requires |a| >= 1 && |R_a| >= 1
+   requires |a| >= 1 && |R_a| >= 1
+  ensures Aux_0(a + R_a) == Aux_0Join(Aux_0(a), Aux_0(R_a))
+  {
+    if |R_a| == 1 
+    {
+    assert(a + R_a == a + [R_a[0]]);
+    
+     } else {
+    calc{
+    Aux_0(a + R_a);
+    =={ assert(a + R_a[..|R_a|-1]) + [R_a[|R_a|-1]] == a + R_a; }
+    Aux_0Join(Aux_0(a), Aux_0(R_a));
+    } // End calc.
+  } // End else.
+} // End lemma.
+
+lemma BaseCaseIss(a : seq<int>, R_a : seq<int>)
+  requires |a| >= 1 && |R_a| >= 1
+  
+  requires |a| >= 1 && |R_a| >= 1
+  ensures Iss(a) == IssJoin(Aux_0(a), Prev(a), Iss(a), Aux_0([R_a[0]]), Prev([R_a[0]]), Iss([R_a[0]]))
+  {}
+
+lemma HomIss(a : seq<int>, R_a : seq<int>)
+  requires |a| >= 1 && |R_a| >= 1
+   requires |a| >= 1 && |R_a| >= 1
+  ensures Iss(a + R_a) == IssJoin(Aux_0(a), Prev(a), Iss(a), Aux_0(R_a), Prev(R_a), Iss(R_a))
+  {
+    if R_a == [] 
+    {
+    assert(a + [] == a);
+    BaseCaseIss(a, R_a);
+    
+     } else {
+    calc{
+    Iss(a + R_a);
+    =={
+      HomPrev(a, R_a[..|R_a| - 1]);
+      assert(a + R_a[..|R_a|-1]) + [R_a[|R_a|-1]] == a + R_a;
+      }
+    IssJoin(Aux_0(a), Prev(a), Iss(a), Aux_0(R_a), Prev(R_a), Iss(R_a));
+    } // End calc.
+  } // End else.
+} // End lemma.
+
+lemma BaseCasePrev(a : seq<int>)
+  ensures Prev(a) == PrevJoin(Prev(a), Prev([]))
+  {}
+
+lemma HomPrev(a : seq<int>, R_a : seq<int>)
+  ensures Prev(a + R_a) == PrevJoin(Prev(a), Prev(R_a))
+  {
+    if R_a == [] 
+    {
+    assert(a + [] == a);
+    BaseCasePrev(a);
+    
+     } else {
+    calc{
+    Prev(a + R_a);
+    =={ assert(a + R_a[..|R_a|-1]) + [R_a[|R_a|-1]] == a + R_a; }
+    PrevJoin(Prev(a), Prev(R_a));
+    } // End calc.
+  } // End else.
+} // End lemma.
+
